# 初等代数

## 乘法公式与因式分解

- $(a \pm b)^{2} = a^{2} \pm 2ab + b^{2}$
- $(a + b + c)^{2} = a^{2} + b^{2} + c^{2} + 2ab + 2ac + 2bc$
- $(a \pm b)^{3} = a^{3} \pm 3a^{2}b + 3ab^{2} \pm b^{3}$

---

- $a^{2} - b^{2} = (a + b)(a - b)$
- $a^{3} - b^{3} = (a - b)(a^{2} + ab + b^{2})$
- $a^{3} + b^{3} = (a + b)(a^{2} - ab + b^{2})$
- $a^{n} - b^{n} = (a - b)(a^{n - 1} + a^{n - 2}b + a^{n - 3}b^2 + \cdots  + ab^{n - 2} + b^{n - 1})$

## 指数

- $a^{x} a^{y} = a^{x + y}$
- $\dfrac{a^{x}}{a^{y}} = a^{x - y}$

- $(ab)^{x} = a^{x}b^{x}$
- $(a^{x})^{y} = a^{xy}$

## 对数

- $a^{b} = e^{lna^{b}} = e^{blna}$

- $a^{log_{a}b} = b$
- $log_{a}b^{c} = clog_{a}b$

- $log_{a}(MN) = log_{a}M + log_a{N}$
- $log_{a}\dfrac{M}{N} = log_{a}M - log_{a}N$

- $log_{a}b = \dfrac{log_{c}b}{log_{c}a}$

## 不等式

- 对于 $\forall x$，有 $e^{x} ≥ x + 1$
- 对于 $\forall x ≥ 0$，有 $x ≥ sinx$
- 对于 $\forall x > 0$，有 $x - 1 ≥ lnx$

---

- 设 a > b > 0，n > 0，则 $a^{n} > b^{n}$
- 设 a > b > 0，n 为正整数，则 $\sqrt[n]{a} > \sqrt[n]{b}$

- 设 $\dfrac{a}{b} < \dfrac{c}{d}$，则 $\dfrac{a}{b} < \dfrac{a + c}{b + d} < \dfrac{c}{d}$

---

- 非负数的算数平均值不小于其几何平均值，即

  - $\dfrac{a + b}{2} ≥ \sqrt{ab}$

  - $\dfrac{a + b + c}{3} ≥ \sqrt[3]{abc}$

  - $\dfrac{a_{1} + a_{2} + a_{3} + \cdots + a_{n}}{n} ≥ \sqrt[n]{a_{1}a_{2}a_{3} \cdots a_{n}}$

---

- 绝对值不等式

  - $-|a| ≤ a ≤ |a|$

  - $|a + b| ≤ |a| + |b|$

  - $|a| - |b| ≤ |a - b| ≤ |a| + |b|$

## 数列

### 等差数列

- $a_{n} = a_{1} + (n - 1)d = a_{m} + (n - m)d = dn + (a_{1} - d)，n∈N^{*}$

- $S_{n} = \dfrac{n(a_{1} + a_{n})}{2} = na_{1} + \dfrac{n(n - 1)}{2}d = \dfrac{d}{2}n^{2} - (a_{1} - \dfrac{d}{2})n，n∈N^{*}$

### 等比数列

- $a_{n} = a_{1}q^{n - 1} = a_{m}q^{n - m} \space (a_{1},q ≠ 0)$

- $S_{n}=\begin{cases} \dfrac{a_{1}(1 - q^{n})}{1-q} \space (q ≠ 1), \\ na_{1} \space (q = 1) \end{cases}$

### 裂项相消法

- $\dfrac{1}{n(n + 1)} = \dfrac{1}{n} - \dfrac{1}{n + 1}$
- $\dfrac{1}{n(n + k)} = \dfrac{1}{k} (\dfrac{1}{n} - \dfrac{1}{n + k})$
- $\dfrac{1}{nm(n + k)} = \dfrac{1}{k} (\dfrac{1}{nm} - \dfrac{1}{m(n + k)})$

- $\dfrac{1}{(2n - 1)(2n + 1)} = \dfrac{1}{2} (\dfrac{1}{2n-1} - \dfrac{1}{2n + 1})$
- $\dfrac{1}{n(n + 1)(n + 2)} = \dfrac{1}{2} (\dfrac{1}{n(n + 1)} - \dfrac{1}{(n + 1)(n + 2)})$

---

- $\dfrac{1}{\sqrt{a} + \sqrt{b}} = \dfrac{1}{a - b} (\sqrt{a} - \sqrt{b})$

- $\dfrac{1}{\sqrt{n} + \sqrt{n + 1}} = \sqrt{n + 1} - \sqrt{n}$
- $\dfrac{1}{\sqrt{n} + \sqrt{n + k}} = \dfrac{1}{k} (\sqrt{n + k} - \sqrt{n})$

---

- $a^{k} = \dfrac{1}{a - 1} (a^{k + 1} - a^{k})$

- $n \cdot n! = (n + 1)! - n!$

## 排列、组合和二项式定理
